add Proof sentences, fix coqdoc comments

theories/wfArray.v
@@ -28,23 +28,21 @@ From Stalmarck Require Export PolyListAux.
 From Coq Require Export List.
 From Stalmarck Require Export sTactic.
 
-(*Definition of well formed array and some properties *)
+(** Definition of well formed array and some properties *)
 Section wfArray.
 
-(* Ordered list for list on  rZ *)
-
+(** Ordered list for list on rZ *)
 Definition OlistRz := Olist rZ rZlt.
 
-(* Disjoint list for list on rZ *)
-
+(** Disjoint list for list on rZ *)
 Definition DisjointRz := Disjoint rZ eqRz.
 
-(* To be in a list for rZ with no sign consideration  *)
-
+(** To be in a list for rZ with no sign consideration *)
 Definition InRz := InEq rZ eqRz.
 
 Theorem InEqInv :
  forall (a : rZ) (L : list rZ), InRz a L -> In a L \/ In (rZComp a) L.
+Proof.
 intros a L H'; Elimc H'; clear a L; auto with stalmarck.
 intros a b L; case a; case b; unfold eqRz in |- *; simpl in |- *;
  intros a' b' Eqt; rewrite Eqt; auto with stalmarck.
@@ -52,6 +50,7 @@ intros a b L H' H'0; elim H'0; auto with datatypes stalmarck.
 Qed.
 
 Theorem InRzDec : forall (a : rZ) (L : list rZ), {InRz a L} + {~ InRz a L}.
+Proof.
 intros a L; elim L; auto with stalmarck.
 right; red in |- *; intros H'; inversion H'.
 intros a0 l H'; case H'.
@@ -64,15 +63,15 @@ right; red in |- *; intros H'2; inversion_clear H'2.
 case H'1; auto with stalmarck.
 case H'0; auto with stalmarck.
 Qed.
-(* A vM is either a reference or an equivalence class *)
 
+(** A vM is either a reference or an equivalence class *)
 Inductive vM : Set :=
   | ref : rZ -> vM
   | class : list rZ -> vM.
-(*We can decide on list *)
 
+(** We can decide on list *)
 Definition listDec :
-  forall (A : Set) (eqDec : forall a b : A, {a = b} + {a <> b})
+  forall (A : Type) (eqDec : forall a b : A, {a = b} + {a <> b})
     (L1 L2 : list A), {L1 = L2} + {L1 <> L2}.
 intros A eqDec.
 fix listDec 1.
@@ -88,8 +87,8 @@ left; rewrite Eq0; rewrite Eq1; auto with stalmarck.
 right; Contradict Eq1; inversion Eq1; auto with stalmarck.
 right; Contradict Eq0; inversion Eq0; auto with stalmarck.
 Defined.
-(* We can decide equality on vM *)
 
+(** We can decide equality on vM *)
 Definition vMDec : forall a b : vM, {a = b} + {a <> b}.
 intros a b; case a; case b;
  try (intros; right; red in |- *; intros; discriminate; fail).
@@ -104,24 +103,24 @@ Defined.
 Let get := rArrayGet vM.
 
 Let set := rArraySet vM.
-(*We point always to something smaller *)
 
+(** We point always to something smaller *)
 Inductive pointerDecrease : rArray vM -> Prop :=
     pointerDecreaseDef :
       forall Ar : rArray vM,
       (forall (r : rNat) (s : rZ), get Ar r = ref s -> rVlt s r) ->
       pointerDecrease Ar.
-(* Value of pointers are not pointers *)
 
+(** Value of pointers are not pointers *)
 Inductive pointToClassRef : rArray vM -> Prop :=
     pointToClassRefDef :
       forall Ar : rArray vM,
       (forall (r : rNat) (s t : rZ),
        get Ar r = ref s -> get Ar (valRz s) <> ref t) -> 
       pointToClassRef Ar.
-(* all the elements of an equivalence classe points to the class,
-    and if one element points to an equivalent class it is in the equivalence class *)
 
+(** all the elements of an equivalence classe points to the class,
+    and if one element points to an equivalent class it is in the equivalence class *)
 Inductive pointToClassClass : rArray vM -> Prop :=
     pointToClassClassRef :
       forall Ar : rArray vM,
@@ -130,33 +129,37 @@ Inductive pointToClassClass : rArray vM -> Prop :=
       (forall (r : rNat) (s : rZ) (Ls : list rZ),
        get Ar r = ref s -> get Ar (valRz s) = class Ls -> In (samePol s r) Ls) ->
       pointToClassClass Ar.
-(*Equivalent classes are ordered list *)
 
+(** Equivalent classes are ordered list *)
 Inductive OlistArray : rArray vM -> Prop :=
     OlistArrayDef :
       forall Ar : rArray vM,
       (forall (r : rNat) (Lr : list rZ), get Ar r = class Lr -> OlistRz Lr) ->
       OlistArray Ar.
-(* A  well formed array has all the previous properties.
- The idea is that we want every non minimal elements to point by  Ref to its minimal element
- and the minimal elment to contain by Class the elements pointing to it
- Example: if we have to represent [2=-3;1=3] we have
-           f(1)= Class [-2;3] 
-           f(2) = Ref -1
-           f(3) = Ref 1 
-*)
 
+(** A well formed array has all the previous properties.
+ The idea is that we want every non minimal elements to point by
+ Ref to its minimal element and the minimal elment to contain by
+ Class the elements pointing to it
+
+ Example: if we have to represent [2=-3;1=3] we have
+
+ - f(1)= Class [-2;3] 
+ - f(2) = Ref -1
+ - f(3) = Ref 1 
+*)
 Inductive wellFormedArray : rArray vM -> Prop :=
     wellFormedArrayDef :
       forall (Ar : rArray vM) (pD : pointerDecrease Ar)
         (pR : pointToClassRef Ar) (pC : pointToClassClass Ar)
         (oC : OlistArray Ar), wellFormedArray Ar.
-(* Well formedness is compatible with equality *)
 
+(** Well formedness is compatible with equality *)
 Theorem WarCompEq :
  forall Ar1 Ar2 : rArray vM,
  (forall a : rNat, get Ar1 a = get Ar2 a) ->
  wellFormedArray Ar1 -> wellFormedArray Ar2.
+Proof.
 intros Ar1 Ar2 H' War1; inversion War1.
 apply wellFormedArrayDef; auto with stalmarck.
 apply pointerDecreaseDef; auto with stalmarck.
@@ -176,13 +179,14 @@ intros r Lr; repeat rewrite <- H'; auto with stalmarck.
 intros H'0; inversion oC; auto with stalmarck.
 apply H0 with (r := r); auto with stalmarck.
 Qed.
+
 Variable Ar : rArray vM.
 Hypothesis War : wellFormedArray Ar.
-(*******************************************
-  Inversion theorems for WellformedArray 
-********************************************)
+
+(** Inversion theorems for WellformedArray *)
 
 Theorem wfPd : forall (r : rNat) (t : rZ), get Ar r = ref t -> rVlt t r.
+Proof.
 intros r t H'; inversion War.
 inversion pD.
 apply H0 with (1 := H'); auto with stalmarck.
@@ -190,6 +194,7 @@ Qed.
 
 Theorem wfPcr :
  forall (r : rNat) (t u : rZ), get Ar r = ref t -> get Ar (valRz t) <> ref u.
+Proof.
 intros r t u H'; inversion War.
 inversion pR; apply H0 with (1 := H'); auto with stalmarck.
 Qed.
@@ -197,6 +202,7 @@ Qed.
 Theorem wfPcc1 :
  forall (r : rNat) (s : rZ) (Lr : list rZ),
  get Ar r = class Lr -> In s Lr -> get Ar (valRz s) = ref (samePol s r).
+Proof.
 intros r s Lr H' H'0; inversion War.
 inversion pC; apply H0 with (1 := H'); auto with stalmarck.
 Qed.
@@ -204,20 +210,23 @@ Qed.
 Theorem wfPcc2 :
  forall (r : rNat) (s : rZ) (Ls : list rZ),
  get Ar r = ref s -> get Ar (valRz s) = class Ls -> In (samePol s r) Ls.
+Proof.
 intros r s Ls H' H'0; inversion War.
 inversion pC; apply H1 with (1 := H') (2 := H'0); auto with stalmarck.
 Qed.
 
 Theorem wfOl :
  forall (r : rNat) (Lr : list rZ), get Ar r = class Lr -> OlistRz Lr.
+Proof.
 intros r Lr H'; inversion War.
 inversion oC; apply H0 with (1 := H'); auto with stalmarck.
 Qed.
-(*** Equivalence classes are disjoint *)
 
+(** Equivalence classes are disjoint *)
 Theorem refSameEq :
  forall (a b : rZ) (r s : rNat),
  ref (samePol a s) = ref (samePol b r) -> s = r.
+Proof.
 intros a b r s; case a; case b; simpl in |- *; intros a1 b1 C1; inversion C1;
  auto with stalmarck.
 Qed.
@@ -225,6 +234,7 @@ Qed.
 Theorem wfDisjoint :
  forall (r s : rNat) (Lr Ls : list rZ),
  s <> r -> get Ar r = class Lr -> get Ar s = class Ls -> DisjointRz Lr Ls.
+Proof.
 intros r s Lr Ls H' H'0 H'1; red in |- *; apply DisjointDef.
 intros a H'2; red in |- *; intros H'3; case H'.
 case (InEqInv _ _ H'2); intros In1; generalize (wfPcc1 _ _ _ H'0 In1);
@@ -241,30 +251,33 @@ case a; simpl in |- *; auto with stalmarck.
 apply refSameEq with (a := rZComp a) (b := rZComp a); rewrite <- get1;
  rewrite <- get2; auto with stalmarck.
 Qed.
-(*There is no loop in the pointers *)
 
+(** There is no loop in the pointers *)
 Theorem getNotIdP : forall r : rZ, get Ar (valRz r) <> ref r.
+Proof.
 intros r; red in |- *; intros H'.
 absurd (rVlt r (valRz r)); auto with stalmarck.
 unfold rVlt in |- *; auto with stalmarck.
 apply wfPd; auto with stalmarck.
 Qed.
-(* The element that contains an equivalence classis smaller than all the element 
- of the class *)
 
+(** The element that contains an equivalence classis smaller than all the element 
+ of the class *)
 Theorem wellFormedArrayInImpLt :
  forall (a : rNat) (b : rZ) (La : list rZ),
  get Ar a = class La -> In b La -> rlt a (valRz b).
+Proof.
 intros a b La geta Inb.
 replace a with (valRz (samePol b a)).
 generalize (wfPd _ _ (wfPcc1 _ _ _ geta Inb)); unfold rVlt in |- *; auto with stalmarck.
 case b; case a; simpl in |- *; auto with stalmarck.
 Qed.
-(* An element that contains an equivalence class can't be in a equivalence class *)
 
+(** An element that contains an equivalence class can't be in a equivalence class *)
 Theorem wellFormedArrayInImpNotEq :
  forall (a b : rNat) (La Lb : list rZ),
  get Ar a = class La -> get Ar b = class Lb -> ~ InRz (rZPlus a) Lb.
+Proof.
 intros a b La Lb geta getb; red in |- *; intros H'3.
 case (InEqInv (rZPlus a) Lb H'3); intros H'4; auto with stalmarck.
 absurd (get Ar (valRz (rZPlus a)) = class La); auto with stalmarck.
@@ -274,45 +287,48 @@ absurd (get Ar (valRz (rZMinus a)) = class La); auto with stalmarck.
 rewrite wfPcc1 with (1 := getb); auto with stalmarck.
 red in |- *; intro; discriminate.
 Qed.
-(*If two elements contains two equivalent classes that are not disjoint these
-  elements are equal *)
 
+(** If two elements contains two equivalent classes that are not disjoint these
+  elements are equal *)
 Theorem wellFormedArrayInBothImpEq :
  forall (a b : rNat) (c d : rZ) (La Lb : list rZ),
  get Ar a = class La ->
  get Ar b = class Lb -> In c La -> In d Lb -> eqRz c d -> a = b.
+Proof.
 intros a b c d La Lb geta getb inc1 inc2 eqRz1.
 apply refSameEq with (a := c) (b := d).
 rewrite <- wfPcc1 with (1 := geta); auto with stalmarck.
 rewrite <- wfPcc1 with (1 := getb); auto with stalmarck.
 rewrite eqRz1; auto with stalmarck.
 Qed.
-(* Same as before but with no sign distinction *)
 
+(** Same as before but with no sign distinction *)
 Theorem wellFormedArrayInRzBothImpEq :
  forall (a b : rNat) (c : rZ) (La Lb : list rZ),
  get Ar a = class La ->
  get Ar b = class Lb -> InRz c La -> InRz c Lb -> a = b.
+Proof.
 intros a b c La Lb H'0 H'1 H'2 H'3.
 case (InEqInv c La H'2); case (InEqInv c Lb H'3); intros H'4 H'5;
  apply
   wellFormedArrayInBothImpEq with (1 := H'0) (2 := H'1) (3 := H'5) (4 := H'4);
  auto with stalmarck.
 Qed.
-(* An element that contains an equivalence class is  not in the class *)
 
+(** An element that contains an equivalence class is  not in the class *)
 Theorem wellFormedArrayInImpNotEqSimpl :
  forall (a : rNat) (La : list rZ),
  get Ar a = class La -> ~ InRz (rZPlus a) La.
 intros a La H'.
 apply wellFormedArrayInImpNotEq with (1 := H') (2 := H'); auto with stalmarck.
 Qed.
-(*If an element is not in an euqivalent class its value can't be the element
-    that contains the equialent class *)
 
+(** If an element is not in an euqivalent class its value can't be the element
+    that contains the equialent class *)
 Theorem wellFormedArrayNInImpNotRef :
  forall (a : rNat) (b : rZ) (L : list rZ),
  get Ar a = class L -> ~ In b L -> get Ar (valRz b) <> ref (samePol b a).
+Proof.
 intros a b L H' H'0; Contradict H'0.
 cut (b = samePol (samePol b a) (valRz b)).
 intros H'1; rewrite H'1.
@@ -321,4 +337,5 @@ rewrite <- H'; unfold get in |- *; auto with stalmarck.
 case b; simpl in |- *; auto with stalmarck.
 case b; simpl in |- *; auto with stalmarck.
 Qed.
+
 End wfArray.
