theories/PolyListAux.v
@@ -24,17 +24,19 @@ From Coq Require Import Arith.
 From Coq Require Import List.
 
 Section Auxrem.
-Variable A : Set.
+Variable A : Type.
 Variable ADec : forall a b : A, {a = b} + {a <> b}.
 
 Theorem NotInCons1 :
  forall (a b : A) (L : list A), ~ In a (b :: L) -> ~ In a L.
+Proof.
 intros a b L H'; red in |- *; intros H'0; apply H'; simpl in |- *; auto.
 Qed.
 
 Theorem map_id :
  forall f : A -> A,
  (forall x : A, f (f x) = x) -> forall L : list A, map f (map f L) = L.
+Proof.
 intros f H' L; elim L; simpl in |- *; auto.
 intros a l H'0.
 rewrite H'; rewrite H'0; auto.
@@ -51,6 +53,7 @@ Fixpoint rem (a : A) (L : list A) {struct L} : list A :=
   end.
 
 Theorem remNotIn : forall (a : A) (L : list A), ~ In a (rem a L).
+Proof.
 intros a L; elim L; simpl in |- *; auto.
 intros a0 l H'; case (ADec a a0); auto.
 intros H'0; red in |- *; intros H'1; case H'1; auto.
@@ -58,6 +61,7 @@ Qed.
 
 Theorem remIn :
  forall (a b : A) (L : list A), In b L -> a <> b -> In b (rem a L).
+Proof.
 intros a b L; elim L; simpl in |- *; auto.
 intros a0 l H' H'0 H'1; case (ADec a a0); case H'0; auto with datatypes.
 intros H'2 H'3; case H'1; rewrite H'3; auto.
@@ -65,6 +69,7 @@ intros H'2; rewrite H'2; auto with datatypes.
 Qed.
 
 Theorem remEq : forall (a : A) (L : list A), ~ In a L -> rem a L = L.
+Proof.
 intros a L; elim L; simpl in |- *; auto.
 intros a0 l H' H'0; case (ADec a a0); auto with datatypes.
 intros H'1; case H'0; auto.
@@ -73,6 +78,7 @@ Qed.
 
 Theorem remSizeLess :
  forall (a : A) (L : list A), In a L -> length (rem a L) < length L.
+Proof.
 intros a L; elim L; simpl in |- *; auto.
 intros H'; elim H'.
 intros a0 l H' H'0; case (ADec a a0); simpl in |- *; auto with datatypes.
@@ -81,5 +87,7 @@ intros H'2; rewrite remEq; auto.
 intros H'1; case H'0; auto with arith.
 intros H'2; case H'1; auto.
 Qed.
+
 End Auxrem.
+
 #[export] Hint Resolve remSizeLess remEq remIn remNotIn : core.
