theories/doTriplets.v
@@ -23,8 +23,7 @@ Propagation as transitive closure of the one step propagation
 From Stalmarck Require Export doTriplet.
 From Stalmarck Require Import PolyListAux.
 
-(* Reflexive transitive closure of doTriplet *)
-
+(** Reflexive transitive closure of doTriplet *)
 Inductive doTripletsP : State -> list triplet -> State -> Prop :=
   | doTripletsRef :
       forall (S1 S2 : State) (L : list triplet),
@@ -33,12 +32,14 @@ Inductive doTripletsP : State -> list triplet -> State -> Prop :=
       forall (S1 S2 S3 : State) (L : list triplet) (t : triplet),
       In t L ->
       doTripletP S1 t S2 -> doTripletsP S2 L S3 -> doTripletsP S1 L S3.
-#[export] Hint Resolve doTripletsRef : stalmarck.
-(* It is compatible *)
 
+#[export] Hint Resolve doTripletsRef : stalmarck.
+
+(** It is compatible *)
 Theorem doTripletsComp :
  forall (S1 S2 S3 S4 : State) (L : list triplet),
  doTripletsP S1 L S2 -> eqState S3 S1 -> eqState S4 S2 -> doTripletsP S3 L S4.
+Proof.
 intros S1 S2 S3 S4 L H'; generalize S3 S4; elim H'; clear H' L S1 S2 S3 S4;
  auto with stalmarck.
 intros S1 S2 L H' S3 S4 H'0 H'1.
@@ -51,22 +52,24 @@ elim (doTripletEqCompEx S1 S2 S0 t);
  auto with stalmarck.
 apply doTripletsTrans with (S2 := S6) (t := t); auto with stalmarck.
 Qed.
-(* Transitive *)
 
+(** Transitive *)
 Theorem doTripletsRTrans :
  forall (S1 S2 S3 : State) (L : list triplet),
  doTripletsP S1 L S2 -> doTripletsP S2 L S3 -> doTripletsP S1 L S3.
+Proof.
 intros S1 S2 S3 L H'; elim H'; auto with stalmarck.
 intros S4 S5 L0 H'0 H'1.
 apply doTripletsComp with (S1 := S5) (S2 := S3); auto with stalmarck.
 intros S4 S5 S0 L0 t H'0 H'1 H'2 H'3 H'4.
 apply doTripletsTrans with (S2 := S5) (t := t); auto with stalmarck.
 Qed.
-(*We only add equation *)
 
+(** We only add equation *)
 Theorem doTripletsUnionEx :
  forall (S1 S2 : State) (L : list triplet),
  doTripletsP S1 L S2 -> exists S3 : State, eqState S2 (unionState S3 S1).
+Proof.
 intros S1 S2 L H'; elim H'; auto with stalmarck.
 intros S3 S4 H'0 H'1; exists S3; auto with stalmarck.
 apply eqStateTrans with (S2 := S3); auto with stalmarck.
@@ -79,20 +82,22 @@ apply eqStateTrans with (S2 := unionState S7 S4); auto with stalmarck.
 rewrite E; auto with stalmarck.
 apply unionStateAssoc; auto with stalmarck.
 Qed.
-(* The state always grows *)
 
+(** The state always grows *)
 Theorem doTripletsIncl :
  forall (S1 S2 : State) (L : list triplet),
  doTripletsP S1 L S2 -> inclState S1 S2.
+Proof.
 intros S1 S2 L H'.
 elim (doTripletsUnionEx S1 S2 L); [ intros S3 E | idtac ]; auto with stalmarck.
 apply inclStateEqStateComp with (S1 := S1) (S3 := unionState S3 S1); auto with stalmarck.
 Qed.
-(* It is a congruence *)
 
+(** It is a congruence *)
 Theorem doTripletCongruent :
  forall (S1 S2 S3 : State) (L : list triplet),
  doTripletsP S1 L S2 -> doTripletsP (unionState S3 S1) L (unionState S3 S2).
+Proof.
 intros S1 S2 S3 L H'; Elimc H'; clear S1 S2 L; auto with stalmarck.
 intros S1 S2 S0 L t H' H'0 H'1 H'2.
 apply doTripletsRTrans with (S2 := unionState S3 S2); auto with stalmarck.
@@ -102,12 +107,13 @@ elim (doTripletCongruentEx S1 S2 S3 t);
 apply doTripletsRTrans with (S2 := S4); auto with stalmarck.
 apply doTripletsTrans with (S2 := S4) (t := t); auto with stalmarck.
 Qed.
-(* It is monotone *)
 
+(** It is monotone *)
 Theorem doTripletsMonotoneEx :
  forall (S1 S2 S3 : State) (L : list triplet),
  doTripletsP S1 L S3 ->
  inclState S1 S2 -> exists S4 : State, doTripletsP S2 L S4 /\ inclState S3 S4.
+Proof.
 intros S1 S2 S3 L H' H'0.
 lapply (doTripletCongruent S1 S3 S2 L); [ intros H'5 | idtac ]; auto with stalmarck.
 exists (unionState S2 S3); split; auto with stalmarck.
@@ -115,13 +121,14 @@ apply doTripletsComp with (S1 := unionState S2 S1) (S2 := unionState S2 S3);
  auto with stalmarck.
 red in |- *; split; auto with stalmarck.
 Qed.
-(* It is confluent *)
 
+(** It is confluent *)
 Theorem doTripletsConftEx :
  forall (L : list triplet) (S1 S2 S3 : State),
  doTripletsP S1 L S2 ->
  doTripletsP S1 L S3 ->
  exists S4 : State, doTripletsP S2 L S4 /\ doTripletsP S3 L S4.
+Proof.
 intros L S1 S2 S3 H' H'0.
 elim (doTripletsUnionEx S1 S2 L); [ intros S4 E | idtac ]; auto with stalmarck.
 elim (doTripletsUnionEx S1 S3 L); [ intros S5 E0 | idtac ]; auto with stalmarck.
@@ -141,13 +148,14 @@ apply doTripletsComp with (S1 := unionState S5 S1) (S2 := unionState S5 S2);
  auto with stalmarck.
 apply doTripletCongruent; auto with stalmarck.
 Qed.
-(* We don't loose realizability of memories if the triplets are realized *)
 
+(** We don't lose realizability of memories if the triplets are realized *)
 Theorem doTripletsRealizeStateEval :
  forall (f : rNat -> bool) (S1 S2 : State) (L : list triplet),
  realizeState f S1 ->
  doTripletsP S1 L S2 ->
  realizeTriplets f L -> f zero = true -> realizeState f S2.
+Proof.
 intros f S1 S2 L H' H'0; generalize H'; elim H'0; auto with stalmarck.
 intros S3 S4 L0 H'1 H'2 H'3 H'4.
 apply realizeStateIncl with (S1 := S3); auto with stalmarck; inversion H'1; auto with stalmarck.
@@ -166,6 +174,7 @@ Theorem doTripletsTermExAux :
     (exists S4 : State,
        doTripletsP S1 (rem _ tripletDec t L) S3 /\
        doTripletP S3 t S4 /\ doTripletsP S4 (rem _ tripletDec t L) S2)).
+Proof.
 intros L S1 S2 H'; Elimc H'; clear L S1 S2; auto with stalmarck.
 intros S1 S2 S3 L t H' H'0 H'1 H'2 t0 H'3.
 case (tripletDec t t0); intros H.
@@ -195,8 +204,8 @@ apply doTripletsTrans with (S2 := S2) (t := t); auto with stalmarck.
 right; exists S0; exists S4; split; [ idtac | split ]; auto with stalmarck.
 apply doTripletsTrans with (S2 := S2) (t := t); auto with stalmarck.
 Qed.
-(* Once we have used  a triplet we can do without *)
 
+(** Once we have used  a triplet we can do without *)
 Theorem doTripletsTermEx :
  forall (L : list triplet) (S1 S2 : State),
  doTripletsP S1 L S2 ->
@@ -205,6 +214,7 @@ Theorem doTripletsTermEx :
     (exists S3 : State,
        In t L /\
        doTripletP S1 t S3 /\ doTripletsP S3 (rem _ tripletDec t L) S2)).
+Proof.
 intros L S1 S2 H'; inversion H'; auto with stalmarck.
 right; exists t; exists S3; split; try split; auto with stalmarck.
 lapply (doTripletsTermExAux L S3 S2);
@@ -219,11 +229,12 @@ apply doTripletsComp with (S1 := S6) (S2 := S2); auto with stalmarck.
 apply doTripletInvol with (t := t) (S1 := S1) (S2 := S3); auto with stalmarck.
 apply doTripletsIncl with (L := rem triplet tripletDec t L); auto with stalmarck.
 Qed.
-(* The more we have triplets the more we can do *)
 
+(** The more we have triplets the more we can do *)
 Theorem doTripletsInclList :
  forall (L1 L2 : list triplet) (S1 S2 : State),
  incl L1 L2 -> doTripletsP S1 L1 S2 -> doTripletsP S1 L2 S2.
+Proof.
 intros L1 L2 S1 S2 H' H'0; generalize L2 H'; elim H'0; clear H'0 H' L2; auto with stalmarck.
 intros S3 S4 S5 L0 t H' H'0 H'1 H'2 L2 H'3.
 apply doTripletsTrans with (S2 := S4) (t := t); auto with datatypes stalmarck.
