theories/ltState.v
@@ -31,36 +31,39 @@ From Coq Require Import Relation_Definitions.
 Section lt.
 Variable L : list rNat.
 
-(* returns 0 if a=b 1 otherwise *)
-
+(** returns 0 if a=b, 1 otherwise *)
 Definition oneState (S : State) (a b : rZ) :=
   match eqStateRzDec S a b with
   | left _ => 0
   | right _ => 1
   end.
-(* oneState is monotone for inclusion *)
 
+(** [oneState] is monotone for inclusion *)
 Theorem oneStateLe :
  forall (a b : rZ) (S1 S2 : State),
  inclState S1 S2 -> oneState S2 a b <= oneState S1 a b.
+Proof.
 intros a b S1 S2 H'; unfold oneState in |- *.
 case (eqStateRzDec S1 a b); case (eqStateRzDec S2 a b); auto with stalmarck.
 intros H'0 H'1; case H'0; auto with stalmarck.
 Qed.
-Local Hint Resolve oneStateLe : stalmarck.
-(* It is strict if inclusion is strict *)
 
+#[local] Hint Resolve oneStateLe : stalmarck.
+
+(** It is strict if inclusion is strict *)
 Theorem oneStateLt :
  forall (a b : rZ) (S1 S2 : State),
  inclState S1 S2 ->
  eqStateRz S2 a b -> ~ eqStateRz S1 a b -> oneState S2 a b < oneState S1 a b.
+Proof.
 intros a b S1 S2 H'; unfold oneState in |- *.
 case (eqStateRzDec S1 a b); case (eqStateRzDec S2 a b); auto with stalmarck.
 intros H'0 H'1 H'2 H'3; case H'3; auto with stalmarck.
 intros H'0 H'1 H'2 H'3; case H'0; auto with stalmarck.
 intros H'0 H'1 H'2 H'3; case H'0; auto with stalmarck.
 Qed.
-Local Hint Resolve oneStateLt : stalmarck.
+
+#[local] Hint Resolve oneStateLt : stalmarck.
 
 (* Returns 1 if +/- a = +/- b (if the state is not contradictory then 4), O otherwise *)
 
@@ -69,70 +72,83 @@ Definition oneStateAll (S : State) (a b : rNat) :=
   (oneState S (rZMinus a) (rZPlus b) + oneState S (rZMinus a) (rZMinus b)).
 
 Theorem lePlusComp : forall a b c d : nat, a <= b -> c <= d -> a + c <= b + d.
+Proof.
 intros a b c d H' H'0.
 apply Nat.le_trans with (m := a + d); auto with stalmarck.
 apply Nat.add_le_mono_l; auto with stalmarck.
 apply Nat.add_le_mono_r; auto with stalmarck.
 Qed.
-Local Hint Resolve lePlusComp : stalmarck.
-(* Monotonicity *)
 
+#[local] Hint Resolve lePlusComp : stalmarck.
+
+(** Monotonicity *)
 Theorem oneStateAllLe :
  forall (a b : rNat) (S1 S2 : State),
  inclState S1 S2 -> oneStateAll S2 a b <= oneStateAll S1 a b.
+Proof.
 intros a b S1 S2 H'; unfold oneStateAll in |- *; generalize oneStateLe;
  intros H'1; auto with stalmarck.
 Qed.
-Local Hint Resolve oneStateAllLe : stalmarck.
+
+#[local] Hint Resolve oneStateAllLe : stalmarck.
 
 Theorem ltlePlusCompL :
  forall a b c d : nat, a < b -> c <= d -> a + c < b + d.
+Proof.
 intros a b c d H' H'0; apply Nat.lt_le_trans with (m := b + c); auto with stalmarck.
 apply Nat.add_lt_mono_r; auto with stalmarck.
 Qed.
-Local Hint Resolve ltlePlusCompL : stalmarck.
+
+#[local] Hint Resolve ltlePlusCompL : stalmarck.
 
 Theorem ltlePlusCompR :
  forall a b c d : nat, a <= b -> c < d -> a + c < b + d.
+Proof.
 intros a b c d H' H'0; apply Nat.le_lt_trans with (m := b + c); auto with stalmarck.
 apply Nat.add_lt_mono_l; auto with stalmarck.
 Qed.
-Local Hint Resolve ltlePlusCompR : stalmarck.
-(* Strict monotony *)
 
+#[local] Hint Resolve ltlePlusCompR : stalmarck.
+
+(** Strict monotony *)
 Theorem oneStateAllLt :
  forall (a b : rZ) (S1 S2 : State),
  inclState S1 S2 ->
  eqStateRz S2 a b ->
  ~ eqStateRz S1 a b ->
  oneStateAll S2 (valRz a) (valRz b) < oneStateAll S1 (valRz a) (valRz b).
+Proof.
 intros a b S1 S2 H'; unfold oneStateAll in |- *.
 case a; case b; simpl in |- *; auto with stalmarck.
 Qed.
-Local Hint Resolve oneStateAllLt : stalmarck.
-(* Adds oneStateAll for a list of variable *)
 
+#[local] Hint Resolve oneStateAllLt : stalmarck.
+
+(** Adds oneStateAll for a list of variable *)
 Fixpoint Nrel (S1 : State) (a : rNat) (L1 : list rNat) {struct L1} : nat :=
   match L1 with
   | nil => 0
   | b :: L2 => oneStateAll S1 a b + Nrel S1 a L2
   end.
-(* Monotony *)
 
+(** Monotony *)
 Theorem NrelLe :
  forall (L1 : list rNat) (a : rNat) (S1 S2 : State),
  inclState S1 S2 -> Nrel S2 a L1 <= Nrel S1 a L1.
+Proof.
 intros L1 a S1 S2 H'; elim L1; simpl in |- *; auto with stalmarck.
 Qed.
-Local Hint Resolve NrelLe : stalmarck.
-(* Strict monotony *)
 
+#[local] Hint Resolve NrelLe : stalmarck.
+
+(** Strict monotony *)
 Theorem NrelLt :
  forall (L1 : list rNat) (a : rNat) (b : rZ) (S1 S2 : State),
  inclState S1 S2 ->
  eqStateRz S2 (rZPlus a) b ->
  ~ eqStateRz S1 (rZPlus a) b ->
  In (valRz b) L1 -> Nrel S2 a L1 < Nrel S1 a L1.
+Proof.
 intros L1; elim L1; simpl in |- *; auto with stalmarck.
 intros a b S1 S2 H' H'0 H'1 H'2; elim H'2; auto with stalmarck.
 intros a l H' a0 b S1 S2 H'0 H'1 H'2 H'3; Elimc H'3; intros H'3; auto with stalmarck.
@@ -145,9 +161,10 @@ change
 apply ltlePlusCompR; auto with stalmarck.
 apply H' with (b := b); auto with stalmarck.
 Qed.
-Local Hint Resolve NrelLt : stalmarck.
-(* We do a product between two list*)
 
+#[local] Hint Resolve NrelLt : stalmarck.
+
+(** We do a product between two lists *)
 Fixpoint Ncount (S1 : State) (L2 L1 : list rNat) {struct L1} : nat :=
   match L1 with
   | nil => 0
@@ -157,9 +174,11 @@ Fixpoint Ncount (S1 : State) (L2 L1 : list rNat) {struct L1} : nat :=
 Theorem NcountLe :
  forall (L1 L2 : list rNat) (S1 S2 : State),
  inclState S2 S1 -> Ncount S1 L2 L1 <= Ncount S2 L2 L1.
+Proof.
 intros L1; elim L1; simpl in |- *; auto with stalmarck.
 Qed.
-Local Hint Resolve NcountLe : stalmarck.
+
+#[local] Hint Resolve NcountLe : stalmarck.
 
 Theorem NcountLt :
  forall (L1 L2 : list rNat) (a : rNat) (b : rZ),
@@ -169,6 +188,7 @@ Theorem NcountLt :
  inclState S1 S2 ->
  eqStateRz S2 (rZPlus a) b ->
  ~ eqStateRz S1 (rZPlus a) b -> Ncount S2 L2 L1 < Ncount S1 L2 L1.
+Proof.
 intros L1; elim L1; simpl in |- *; auto with stalmarck.
 intros L2 a b H'; elim H'; auto with stalmarck.
 intros a l H' L2 a0 b H'0; Elimc H'0; intros H'0; [ rewrite <- H'0 | idtac ];
@@ -181,17 +201,18 @@ apply ltlePlusCompR; auto with stalmarck.
 apply H' with (a := a0) (b := b); auto with stalmarck.
 Qed.
 
-(* The value of a state is then the number of non-trivial equations that are not valid *)
-
+(** The value of a state is then the number of non-trivial equations that are not valid *)
 Definition valState (S : State) := Ncount S L L.
 
 Theorem vallStateLe :
  forall S1 S2 : State, inclState S1 S2 -> valState S2 <= valState S1.
+Proof.
 unfold valState in |- *; auto with stalmarck.
 Qed.
-Local Hint Resolve vallStateLe : stalmarck.
-(* This number decreases for strict inclusion *)
 
+#[local] Hint Resolve vallStateLe : stalmarck.
+
+(** This number decreases for strict inclusion *)
 Theorem vallStateLt :
  forall a b : rZ,
  In (valRz a) L ->
@@ -208,11 +229,11 @@ generalize H'0; case b; auto with stalmarck.
 apply eqStateRzSym; auto with stalmarck.
 Qed.
 
-(* Using valState and lt we get our order *)
-
+(** Using [valState] and [lt] we get our order *)
 Definition ltState (S1 S2 : State) := valState S1 < valState S2.
 
 Theorem ltStateTrans : transitive State ltState.
+Proof.
 red in |- *; unfold ltState in |- *; auto with stalmarck.
 intros S1 S2 S3 H' H'0.
 apply Nat.lt_trans with (m := valState S2); auto with stalmarck.
@@ -221,6 +242,7 @@ Qed.
 Theorem ltStateEqComp :
  forall S1 S2 S3 S4 : State,
  eqState S1 S3 -> eqState S2 S4 -> ltState S1 S2 -> ltState S3 S4.
+Proof.
 unfold eqState, ltState in |- *.
 intros S1 S2 S3 S4 H' H'0 H'1.
 Elimc H'0; intros H'0 H'2.
@@ -235,13 +257,16 @@ Theorem ltStateLt :
  In (valRz b) L ->
  forall S1 S2 : State,
  inclState S1 S2 -> eqStateRz S2 a b -> ~ eqStateRz S1 a b -> ltState S2 S1.
+Proof.
 intros a b H' H'0 S1 S2 H'1 H'2 H'3; red in |- *.
 apply vallStateLt with (a := a) (b := b); auto with stalmarck.
 Qed.
-(* It is well founded *)
 
+(** It is well founded *)
 Theorem ltStateWf : well_founded ltState.
+Proof.
 unfold ltState in |- *; apply wf_inverse_image with (B := nat); auto with stalmarck.
 try exact lt_wf.
 Qed.
+
 End lt.
