theories/restrictState.v
@@ -24,11 +24,11 @@ of the triplets matter
 From Stalmarck Require Import stalmarck.
 From Stalmarck Require Import ltState.
 
-(* Inversion theorem for contradictory state *)
-
+(** Inversion theorem for contradictory state *)
 Theorem contradictoryAddEq :
  forall (S : State) (a b : rZ),
  contradictory (addEq (a, b) S) -> eqStateRz S a (rZComp b).
+Proof.
 intros S a b H'; cut (eqConstrState (addEq (a, b) S) a (rZComp a)).
 unfold addEq in |- *; intros H'1; inversion H'1; auto with stalmarck;
  try (apply eqStateRzContr with (a := a); auto with stalmarck; fail).
@@ -37,10 +37,12 @@ Elimc H'; intros a0 E.
 apply eqStateRzPImpeqConstrState.
 apply eqStateRzContr with (a := a0); auto with stalmarck.
 Qed.
+
 #[export] Hint Resolve contradictoryAddEq : stalmarck.
 
 Theorem prodRzInL :
  forall (a b : rZ) (L1 L2 : list rZ), In (a, b) (prodRz L1 L2) -> In a L1.
+Proof.
 intros a b L1; elim L1; simpl in |- *; auto with stalmarck.
 intros a0 l H' L2 H'0.
 case (in_app_or _ _ _ H'0); auto with stalmarck.
@@ -53,6 +55,7 @@ Qed.
 
 Theorem prodRzInR :
  forall (a b : rZ) (L1 L2 : list rZ), In (a, b) (prodRz L1 L2) -> In b L2.
+Proof.
 intros a b L1; elim L1; simpl in |- *; auto with stalmarck.
 intros L2 H'; elim H'; auto with stalmarck.
 intros a0 l H' L2 H'0.
@@ -60,8 +63,8 @@ case (in_app_or _ _ _ H'0); auto with stalmarck.
 elim L2; simpl in |- *; auto with stalmarck.
 intros a1 l0 H'1 H'2; Elimc H'2; intros H'2; [ inversion H'2 | idtac ]; auto with stalmarck.
 Qed.
-(* We remove in the second list the element that are not in the first *)
 
+(** We remove in the second list the element that are not in the first *)
 Fixpoint stripInRz (L : list rNat) (L1 : list rZ) {struct L1} : 
  list rZ :=
   match L1 with
@@ -76,6 +79,7 @@ Fixpoint stripInRz (L : list rNat) (L1 : list rZ) {struct L1} :
 Theorem stripInRzIn1 :
  forall (L : list rNat) (L1 : list rZ) (a : rZ),
  In a (stripInRz L L1) -> In (valRz a) L.
+Proof.
 intros L L1; elim L1; simpl in |- *; auto with stalmarck.
 intros a H'; elim H'; auto with stalmarck.
 intros a l H' a0.
@@ -86,6 +90,7 @@ Qed.
 Theorem stripInRzIn :
  forall (L : list rNat) (L1 : list rZ) (a : rZ),
  In a L1 -> In (valRz a) L -> In a (stripInRz L L1).
+Proof.
 intros L L1; elim L1; simpl in |- *; auto with stalmarck.
 intros a l H' a0 H'0; Elimc H'0; intros H'0; [ rewrite <- H'0 | idtac ];
  case (In_dec rNatDec (valRz a) L); simpl in |- *; 
@@ -93,9 +98,8 @@ intros a l H' a0 H'0; Elimc H'0; intros H'0; [ rewrite <- H'0 | idtac ];
 intros H'1 H'2; case H'1; auto with stalmarck.
 Qed.
 
-(* The restriction of the state is all the non-trival equation of the state
+(** The restriction of the state is all the non-trival equation of the state
      whose elements are in the list *)
-
 Definition restrictState (S : State) (L : list rNat) : State :=
   match eqStateRzContrDec S with
   | left _ => (rZTrue, rZFalse) :: nil
@@ -103,11 +107,13 @@ Definition restrictState (S : State) (L : list rNat) : State :=
       stripRzDec S
         (prodRz (stripInRz L (stripRz S)) (stripInRz L (stripRz S)))
   end.
-(* It seems that this speeds up Coq *)
+
+(** It seems that this speeds up Coq *)
 Opaque eqStateRzContrDec.
 
 Theorem restrictStateIncl :
  forall (S : State) (L : list rNat), inclState (restrictState S L) S.
+Proof.
 intros S L; unfold restrictState in |- *.
 case (eqStateRzContrDec S); auto with stalmarck.
 intros H'; red in |- *; auto with stalmarck.
@@ -120,6 +126,7 @@ apply
 Qed.
 
 Lemma andSym : forall A B : Prop, A /\ B -> B /\ A.
+Proof.
 intuition.
 Qed.
 
@@ -129,6 +136,7 @@ Theorem InState :
  forall a b : rZ,
  eqStateRz S a b ->
  a <> b -> ~ contradictory S -> In (valRz a) L /\ In (valRz b) L.
+Proof.
 intros S L H' a b H'0; generalize H'; Elimc H'0; clear H' S a b; auto with stalmarck.
 intros a S H' H'0; case H'0; auto with stalmarck.
 intros a b S H' H'0 H'1 H'2 H'3.
@@ -157,6 +165,7 @@ Qed.
 Theorem restrictContradiction :
  forall (S : State) (L : list rNat),
  contradictory S <-> contradictory (restrictState S L).
+Proof.
 intros S L; red in |- *; split; auto with stalmarck.
 unfold restrictState in |- *; case (eqStateRzContrDec S); auto with stalmarck.
 intros H' H'0; red in |- *; exists rZTrue; auto with stalmarck; auto with stalmarck.
@@ -174,6 +183,7 @@ Theorem InRestrictState :
  forall (S : State) (L : list rNat) (a b : rZ),
  eqStateRz (restrictState S L) a b ->
  a <> b -> ~ contradictory S -> In (valRz a) L /\ In (valRz b) L.
+Proof.
 intros S L a b H' H'0 H'1.
 apply InState with (S := restrictState S L); auto with stalmarck.
 2: assert (H'3:=restrictContradiction S L); red in H'3; auto with stalmarck.
@@ -198,6 +208,7 @@ Theorem vallStateLtNEq :
  inclState S1 S2 ->
  eqState (restrictState S2 L) S2 ->
  ~ contradictory S2 -> ~ eqState S1 S2 -> valState L S2 < valState L S1.
+Proof.
 intros L S1 S2 H' H'0 Contr0 H'1.
 elim (inclStateDecBis S2 S1); intros H'2; auto with stalmarck.
 case H'1; red in |- *; auto with stalmarck.
@@ -216,6 +227,7 @@ Theorem restrictStateComp :
  forall (S : State) (L : list rNat) (a b : rZ),
  In (valRz a) L ->
  In (valRz b) L -> eqStateRz S a b -> eqStateRz (restrictState S L) a b.
+Proof.
 intros S L a b H' H'0 H'1.
 unfold restrictState in |- *.
 case (eqStateRzContrDec S).
@@ -234,8 +246,7 @@ apply stripInRzIn; auto with stalmarck.
 apply eqConstrStateInR with (a := a); auto with stalmarck.
 Qed.
 
-(* Gives the variable in a triplet*)
-
+(** Gives the variable in a triplet *)
 Definition ResTriplet (t : triplet) : list rNat :=
   match t with
   | Triplet _ v1 v2 v3 => valRz v1 :: valRz v2 :: valRz v3 :: zero :: nil
@@ -248,6 +259,7 @@ Theorem RestrictAddEq1 :
  In zero L ->
  inclState (addEq (a, b) (restrictState S L))
    (restrictState (addEq (a, b) S) L).
+Proof.
 intros S L a b H' H'0 H'1.
 apply inclStateIn; auto with stalmarck.
 simpl in |- *; auto with stalmarck.
@@ -279,6 +291,7 @@ Qed.
 Theorem restrictStateInZeroL :
  forall (S : State) (L : list rNat) (a b : rZ),
  In zero L -> In (a, b) (restrictState S L) -> In (valRz a) L.
+Proof.
 intros S L a b H'; unfold restrictState in |- *.
 case (eqStateRzContrDec S); simpl in |- *; auto with stalmarck.
 intros H'0 H'1; Elimc H'1; intros H'1; inversion H'1; auto with stalmarck.
@@ -291,6 +304,7 @@ Qed.
 Theorem restrictStateInZeroR :
  forall (S : State) (L : list rNat) (a b : rZ),
  In zero L -> In (a, b) (restrictState S L) -> In (valRz b) L.
+Proof.
 intros S L a b H'; unfold restrictState in |- *.
 case (eqStateRzContrDec S); simpl in |- *; auto with stalmarck.
 intros H'0 H'1; Elimc H'1; intros H'1; inversion H'1; auto with stalmarck.
@@ -307,6 +321,7 @@ Theorem RestrictAddEq2 :
  In zero L ->
  inclState (restrictState (addEq (a, b) S) L)
    (addEq (a, b) (restrictState S L)).
+Proof.
 intros S L a b H' H'0 Eqz; apply inclStateIn; auto with stalmarck.
 intros a0 b0 H'1.
 cut (eqConstrState (addEq (a, b) S) a0 b0).
@@ -352,8 +367,8 @@ apply eqStateRzPImpeqConstrState; auto with stalmarck.
 apply eqStateIncl with (S1 := restrictState (addEq (a, b) S) L); auto with stalmarck.
 apply restrictStateIncl; auto with stalmarck.
 Qed.
-(* If the variable of the addition are in the list restriction commutrs with addition *)
 
+(** If the variable of the addition are in the list restriction commutrs with addition *)
 Theorem RestrictAddEq :
  forall (S : State) (L : list rNat) (a b : rZ),
  In (valRz a) L ->
@@ -361,6 +376,7 @@ Theorem RestrictAddEq :
  In zero L ->
  eqState (restrictState (addEq (a, b) S) L)
    (addEq (a, b) (restrictState S L)).
+Proof.
 intros S L a b H' H'0 H'1; red in |- *; split.
 apply RestrictAddEq2; auto with stalmarck.
 apply RestrictAddEq1; auto with stalmarck.
@@ -382,6 +398,7 @@ Theorem doTripletRestrictAux1 :
    (fun S' : State =>
     doTripletP (restrictState S L) t S' /\
     eqState (restrictState (addEq (p, q) (addEq (r, s) S)) L) S').
+Proof.
 intros S t L p1 q1 p q r s H' H'0 H'1 H'2 H'3 H'4 H'5 H'6;
  exists (addEq (p, q) (addEq (r, s) (restrictState S L))); 
  split; auto with stalmarck.
@@ -406,19 +423,21 @@ Theorem doTripletRestrictAux2 :
    (fun S' : State =>
     doTripletP (restrictState S L) t S' /\
     eqState (restrictState (addEq (p, q) S) L) S').
+Proof.
 intros S t L p1 q1 p q H' H'0 H'1 H'2 H'3 H'4;
  exists (addEq (p, q) (restrictState S L)); split; 
  auto with stalmarck.
 apply RestrictAddEq; auto with stalmarck.
 Qed.
-(* If the variable of the triplet are in L, what we can with a state we can do it with its retriction *)
 
+(** If the variable of the triplet are in L, what we can with a state we can do it with its retriction *)
 Theorem doTripletRestrict :
  forall (S1 S2 : State) (t : triplet) (L : list rNat),
  doTripletP S1 t S2 ->
  incl (ResTriplet t) L ->
  exists S3 : State,
    doTripletP (restrictState S1 L) t S3 /\ eqState (restrictState S2 L) S3.
+Proof.
 intros S1 S2 t L H' H'0; inversion H';
  simple apply doTripletRestrictAux1 with (1 := H) ||
    apply doTripletRestrictAux2 with (1 := H); rewrite <- H0 in H'0;
@@ -426,12 +445,13 @@ intros S1 S2 t L H' H'0; inversion H';
  auto with datatypes stalmarck; apply restrictStateComp; repeat rewrite valRzComp;
  auto with datatypes stalmarck.
 Qed.
-(* To restrict is involutive *)
 
+(** To restrict is involutive *)
 Theorem restrictStateInvol :
  forall (S : State) (L : list rNat),
  In zero L ->
  eqState (restrictState S L) (restrictState (restrictState S L) L).
+Proof.
 intros S L H; red in |- *; split; auto with stalmarck.
 2: apply restrictStateIncl; auto with stalmarck.
 apply inclStateIn; auto with stalmarck.
@@ -440,12 +460,13 @@ apply restrictStateComp; auto with stalmarck.
 apply restrictStateInZeroL with (S := S) (b := b); auto with stalmarck.
 apply restrictStateInZeroR with (S := S) (a := a); auto with stalmarck.
 Qed.
-(* It is monotone *)
 
+(** It is monotone *)
 Theorem restricMonotone :
  forall (S1 S2 : State) (L1 L2 : list rNat),
  inclState S1 S2 ->
  incl L1 L2 -> inclState (restrictState S1 L1) (restrictState S2 L2).
+Proof.
 intros S1 S2 L1 L2 H' H'0.
 apply inclStateIn; auto with stalmarck.
 intros a b H'1.
@@ -471,11 +492,12 @@ apply eqStateIncl with (S1 := restrictState S1 L1); auto with stalmarck.
 apply restrictStateIncl; auto with stalmarck.
 unfold restrictState in |- *; case (eqStateRzContrDec S1); auto with stalmarck.
 Qed.
-(* It is compatible with the equality *)
 
+(** It is compatible with the equality *)
 Theorem restrictEqComp :
  forall (S1 S2 : State) (L : list rNat),
  eqState S1 S2 -> eqState (restrictState S1 L) (restrictState S2 L).
+Proof.
 intros S1 S2 L H'; red in |- *; split; apply restricMonotone;
  auto with datatypes stalmarck; red in H'; elim H'; auto with stalmarck.
 Qed.
@@ -489,6 +511,7 @@ Theorem restrictDoTripletCompAux1 :
  In zero L ->
  eqState (addEq (p, q) (addEq (r, s) (restrictState S1 L)))
    (restrictState (addEq (p, q) (addEq (r, s) (restrictState S1 L))) L).
+Proof.
 intros S1 L p q r s H' H'0 H'1 H'2 H'3.
 apply
  eqStateTrans with (S2 := restrictState (addEq (p, q) (addEq (r, s) S1)) L);
@@ -523,6 +546,7 @@ Theorem restrictDoTripletCompAux2 :
  In zero L ->
  eqState (addEq (p, q) (restrictState S1 L))
    (restrictState (addEq (p, q) (restrictState S1 L)) L).
+Proof.
 intros S1 L p q H' H'0 H'1.
 apply eqStateTrans with (S2 := restrictState (addEq (p, q) S1) L); auto with stalmarck.
 apply eqStateTrans with (S2 := addEq (p, q) (restrictState S1 L)); auto with stalmarck.
@@ -536,25 +560,27 @@ apply restrictStateInvol; auto with datatypes stalmarck.
 apply restrictEqComp; auto with stalmarck.
 apply RestrictAddEq; auto with datatypes stalmarck.
 Qed.
-(* If the variables of the triplet are in the restriction, a restricted state stays restricted *)
 
+(** If the variables of the triplet are in the restriction, a restricted state stays restricted *)
 Theorem restrictDoTripletComp :
  forall (S1 S2 : State) (t : triplet) (L : list rNat),
  incl (ResTriplet t) L ->
  doTripletP (restrictState S1 L) t S2 -> eqState S2 (restrictState S2 L).
+Proof.
 intros S1 S2 t L H' H'0; inversion H'0; auto with stalmarck; rewrite <- H0 in H';
  simpl in H';
  apply restrictDoTripletCompAux1 || apply restrictDoTripletCompAux2;
  auto with datatypes stalmarck; repeat rewrite valRzComp; auto with datatypes stalmarck.
 Qed.
-(* What can do the restricted state can be done by the full state *)
 
+(** What can do the restricted state can be done by the full state *)
 Theorem doTripletRestrictInv :
  forall (S1 S2 : State) (t : triplet) (L : list rNat),
  incl (ResTriplet t) L ->
  doTripletP (restrictState S1 L) t S2 ->
  exists S3 : State,
    doTripletP S1 t S3 /\ eqState S3 (unionState (restrictState S2 L) S1).
+Proof.
 intros S1 S2 t L H' H'0.
 elim (doTripletCongruentEx (restrictState S1 L) S2 S1 t);
  [ intros S4 E; Elimc E; intros H'4 H'5 | idtac ]; 
@@ -572,8 +598,8 @@ red in |- *; split; auto with stalmarck.
 apply unionStateMin; auto with stalmarck.
 apply restrictStateIncl; auto with stalmarck.
 Qed.
-(* Returns the list of variables of a list of triplets *)
 
+(** Returns the list of variables of a list of triplets *)
 Fixpoint ResTriplets (L : list triplet) : list rNat :=
   match L with
   | nil => zero :: nil
@@ -581,25 +607,29 @@ Fixpoint ResTriplets (L : list triplet) : list rNat :=
   end.
 
 Theorem zeroInL : forall L : list triplet, In zero (ResTriplets L).
+Proof.
 intros L; elim L; simpl in |- *; auto with datatypes stalmarck.
 Qed.
+
 #[export] Hint Resolve zeroInL : stalmarck.
 
 Theorem ResTripletInResTriplets :
  forall (t : triplet) (L : list triplet),
  In t L -> incl (ResTriplet t) (ResTriplets L).
+Proof.
 intros t L; elim L; simpl in |- *; auto with stalmarck.
 intros H'; elim H'; auto with stalmarck.
 intros a l H' H'0; Elimc H'0; intros H'0; [ rewrite <- H'0 | idtac ];
  auto with datatypes stalmarck.
 Qed.
-(* What can do a state, it can be done by its reduction *)
 
+(** What can do a state, it can be done by its reduction *)
 Theorem doTripletsRestrict :
  forall (S1 S2 : State) (L : list triplet),
  doTripletsP S1 L S2 ->
  doTripletsP (restrictState S1 (ResTriplets L)) L
    (restrictState S2 (ResTriplets L)).
+Proof.
 intros S1 S2 L H'; Elimc H'; clear L S1 S2; auto with stalmarck.
 intros S1 S2 L H'; apply doTripletsRef; auto with stalmarck.
 apply restrictEqComp; auto with stalmarck.
@@ -619,6 +649,7 @@ Theorem restrictDoTripletsCompAux1 :
  forall S3 : State,
  eqState S1 (restrictState S3 (ResTriplets L)) ->
  eqState S2 (restrictState S2 (ResTriplets L)).
+Proof.
 intros S1 S2 L H'; Elimc H'; clear L S1 S2; auto with stalmarck.
 intros S1 S2 L H' S3 H'0.
 apply eqStateTrans with (S2 := S1); auto with stalmarck.
@@ -643,12 +674,12 @@ apply ResTripletInResTriplets; auto with stalmarck.
 apply restrictEqComp; auto with stalmarck.
 Qed.
 
-(* A restricted state gives a restricted state by doTripletsP *)
-
+(** A restricted state gives a restricted state by doTripletsP *)
 Theorem restrictDoTripletsComp :
  forall (S1 S2 : State) (L : list triplet),
  doTripletsP (restrictState S1 (ResTriplets L)) L S2 ->
  eqState S2 (restrictState S2 (ResTriplets L)).
+Proof.
 intros S1 S2 L H'.
 apply
  restrictDoTripletsCompAux1
@@ -656,12 +687,12 @@ apply
  auto with stalmarck.
 Qed.
 
-(* what can be done by a restricted state can be done by the full state *)
-
+(** what can be done by a restricted state can be done by the full state *)
 Theorem doTripletsRestrictInv :
  forall (S1 S2 : State) (L : list triplet),
  doTripletsP (restrictState S1 (ResTriplets L)) L S2 ->
  doTripletsP S1 L (unionState (restrictState S2 (ResTriplets L)) S1).
+Proof.
 intros S1 S2 L H'.
 lapply (restrictDoTripletsComp S1 S2 L); [ intros H'3 | idtac ]; auto with stalmarck.
 apply
@@ -675,15 +706,17 @@ apply unionStateMin; auto with stalmarck.
 apply restrictStateIncl; auto with stalmarck.
 apply eqStateTrans with (S2 := unionState S2 S1); auto with stalmarck.
 Qed.
-(* A restricted state produces always a restricted state *)
 
+(** A restricted state produces always a restricted state *)
 Theorem doTripletsRestrictBis :
  forall (S1 S2 : State) (L : list triplet),
  doTripletsP S1 L S2 ->
  eqState S1 (restrictState S1 (ResTriplets L)) ->
  eqState S2 (restrictState S2 (ResTriplets L)).
+Proof.
 intros S1 S2 L H' H'0.
 apply restrictDoTripletsComp with (S1 := S1); auto with stalmarck.
 apply doTripletsComp with (S1 := S1) (S2 := S2); auto with stalmarck.
 Qed.
+
 Transparent eqStateRzContrDec. 
