theories/stalmarck.v
@@ -24,8 +24,7 @@ From Stalmarck Require Export doTriplets.
 From Stalmarck Require Export interState.
 From Stalmarck Require Export makeTriplet.
 
-(* stalmarck is simply the reflexive transitive closure of dilemma *)
-
+(** stalmarck is simply the reflexive transitive closure of dilemma *)
 Inductive stalmarckP : State -> list triplet -> State -> Prop :=
   | stalmarckPref :
       forall (S1 S2 : State) (L : list triplet),
@@ -38,16 +37,18 @@ Inductive stalmarckP : State -> list triplet -> State -> Prop :=
   | stalmarckTrans :
       forall (S1 S2 S3 : State) (L : list triplet),
       stalmarckP S1 L S2 -> stalmarckP S2 L S3 -> stalmarckP S1 L S3.
+
 #[export] Hint Resolve stalmarckPref : stalmarck.
 
 Definition boolDec : forall a b : bool, {a = b} + {a <> b}.
 intros a b; case a; case b; auto with stalmarck; right; red in |- *; intros; discriminate.
 Defined.
-(* It is compatible with equality *)
 
+(** It is compatible with equality *)
 Theorem stalmarckComp :
  forall (S1 S2 S3 S4 : State) (L : list triplet),
  stalmarckP S1 L S2 -> eqState S3 S1 -> eqState S4 S2 -> stalmarckP S3 L S4.
+Proof.
 intros S1 S2 S3 S4 L H'; generalize S3 S4; Elimc H'; clear L S1 S2 S3 S4.
 intros S1 S2 L H' S3 S4 H'0 H'1.
 apply stalmarckPref; auto with stalmarck.
@@ -58,11 +59,12 @@ apply eqStateTrans with (S2 := S4); auto with stalmarck.
 intros S1 S2 S3 L H' H'0 H'1 H'2 S4 S5 H'3 H'4.
 apply stalmarckTrans with (S2 := S2); auto with stalmarck.
 Qed.
-(* It only adds equations *)
 
+(** It only adds equations *)
 Theorem stalmarckUnionEx :
  forall (S1 S2 : State) (L : list triplet),
  stalmarckP S1 L S2 -> exists S3 : State, eqState S2 (unionState S3 S1).
+Proof.
 intros S1 S2 L H'; Elimc H'; clear L S1 S2; auto with stalmarck.
 exact doTripletsUnionEx.
 intros a b S1 S2 S3 S4 L H' H'0 H'1 H'2 H'3; exists S4; auto with stalmarck.
@@ -101,21 +103,23 @@ apply eqStateTrans with (S2 := unionState S5 (unionState S4 S1)); auto with stal
 apply eqStateTrans with (S2 := unionState S5 S2); auto with stalmarck.
 apply unionStateAssoc; auto with stalmarck.
 Qed.
-(* The state only grows *)
 
+(** The state only grows *)
 Theorem stalmarckIncl :
  forall (S1 S2 : State) (L : list triplet),
  stalmarckP S1 L S2 -> inclState S1 S2.
+Proof.
 intros S1 S2 L H'.
 elim (stalmarckUnionEx S1 S2 L); [ intros S3 E | idtac ]; auto with stalmarck.
 apply inclStateEqStateComp with (S1 := S1) (S3 := unionState S3 S1); auto with stalmarck.
 Qed.
-(* It is  monotone *)
 
+(** It is monotone *)
 Theorem stalmarckMonotoneEx :
  forall (S1 S2 S3 : State) (L : list triplet),
  stalmarckP S1 L S3 ->
  inclState S1 S2 -> exists S4 : State, stalmarckP S2 L S4 /\ inclState S3 S4.
+Proof.
 intros S1 S2 S3 L H'; generalize S2; Elimc H'; auto with stalmarck; clear L S1 S2 S3.
 intros S1 S3 L H' S2 H'0.
 elim (doTripletsMonotoneEx S1 S2 S3 L);
@@ -143,13 +147,14 @@ elim (H'2 S6); [ intros S7 E; elim E; intros H'8 H'9; clear E | idtac ]; auto wi
 exists S7; split; auto with stalmarck.
 apply stalmarckTrans with (S2 := S6); auto with stalmarck.
 Qed.
-(* We don't loose realizability of states if the triplets are realized *)
 
+(** We don't lose realizability of states if the triplets are realized *)
 Theorem stalmarckRealizeStateEval :
  forall (f : rNat -> bool) (S1 S2 : State) (L : list triplet),
  realizeState f S1 ->
  stalmarckP S1 L S2 ->
  realizeTriplets f L -> f zero = true -> realizeState f S2.
+Proof.
 intros f S1 S2 L H' H'0; generalize H'; elim H'0; auto with stalmarck.
 intros S3 S4 L0 H'1 H'2 H'3 H'4.
 apply doTripletsRealizeStateEval with (S1 := S3) (L := L0); auto with stalmarck.
@@ -171,6 +176,7 @@ Theorem stalmarckGivesValidEquation :
  forall (L : list triplet) (a b : rZ) (S : State),
  stalmarckP (addEq (a, rZComp b) nil) L S ->
  contradictory S -> validEquation L a b.
+Proof.
 intros L a b S H' H'0.
 red in |- *; auto with stalmarck.
 intros f H'1 H'2; case (boolDec (rZEval f a) (rZEval f b)); auto with stalmarck.
@@ -181,8 +187,8 @@ apply realizeStateAddEq; auto with stalmarck.
 rewrite rZEvalCompInv; generalize H'3; case (rZEval f a); case (rZEval f b);
  auto with stalmarck; intros H'4; case H'4; auto with stalmarck.
 Qed.
-(* Correctness *)
 
+(** Correctness *)
 Theorem stalmarckCorrect :
  forall (e : Expr) (S : State),
  match makeTriplets (norm e) with
@@ -190,6 +196,7 @@ Theorem stalmarckCorrect :
      stalmarckP (addEq (s, rZFalse) nil) l S ->
      contradictory S -> Tautology e
  end.
+Proof.
 intros e S; generalize (refl_equal (makeTriplets (norm e)));
  pattern (makeTriplets (norm e)) at -2 in |- *; case (makeTriplets (norm e)).
 intros l r r0 H' H'0 H'1.
