theories/state.v
@@ -40,51 +40,58 @@ Inductive eqStateRz : State -> rZ -> rZ -> Prop :=
   | eqStateRzContr :
       forall (a b c : rZ) (S : State),
       eqStateRz S a (rZComp a) -> eqStateRz S b c.
-#[export] Hint Resolve eqStateRzRef eqStateRzIn eqStateRzInv : stalmarck.
-(* equality is compatible with the complement *)
 
+#[export] Hint Resolve eqStateRzRef eqStateRzIn eqStateRzInv : stalmarck.
+
+(** equality is compatible with the complement *)
 Theorem eqStateInvInv :
  forall (S : State) (p q : rZ),
  eqStateRz S (rZComp p) (rZComp q) -> eqStateRz S p q.
+Proof.
 intros S p0 q0 H'; rewrite <- (rZCompInv p0); rewrite <- (rZCompInv q0); auto with stalmarck.
 Qed.
-(* An alternative of eqStateRzContr *)
 
+(** An alternative of eqStateRzContr *)
 Lemma eqStateContr :
  forall (S : State) (p q r s : rZ),
  eqStateRz S p q -> eqStateRz S p (rZComp q) -> eqStateRz S r s.
+Proof.
 intros S p q r s H' H'0.
 apply eqStateRzContr with (a := q); auto with stalmarck.
 apply eqStateRzTrans with (b := p); auto with stalmarck.
 apply eqStateRzSym; auto with stalmarck.
 Qed.
-(* Push complement to the right *)
 
+(** Push complement to the right *)
 Lemma eqStateContrSimpl1 :
  forall (S : State) (p q : rZ),
  eqStateRz S p (rZComp q) -> eqStateRz S (rZComp p) q.
+Proof.
 intros S p q H'.
 apply eqStateInvInv; rewrite rZCompInv; auto with stalmarck.
 Qed.
+
 #[export] Hint Resolve eqStateContrSimpl1 : stalmarck.
 #[export] Hint Immediate eqStateRzSym eqStateInvInv : stalmarck.
 
-(* Adding an equation to a state *)
-
+(** Adding an equation to a state *)
 Definition addEq (p : rZ * rZ) (S : State) : State := p :: S.
-#[export] Hint Unfold addEq : stalmarck.
-(* The added equation is valid *)
 
+#[export] Hint Unfold addEq : stalmarck.
+
+(** The added equation is valid *)
 Lemma eqStateaddEq1 :
  forall (S : State) (p q : rZ), eqStateRz (addEq (p, q) S) p q.
+Proof.
 intros S p q.
 apply eqStateRzIn; simpl in |- *; auto with stalmarck.
 Qed.
-(* All the previous equations are valid *)
 
+(** All the previous equations are valid *)
 Lemma eqStateaddEq2 :
  forall (S : State) (a b p q : rZ),
  eqStateRz S p q -> eqStateRz (addEq (a, b) S) p q.
+Proof.
 intros S a b p q H'; generalize a b; Elimc H'; clear a b p q S; auto with stalmarck.
 intros a b S H' a0 b0; apply eqStateRzIn; simpl in |- *; auto with stalmarck.
 intros a b c S H' H'0 H'1 H'2 a0 b0.
@@ -92,22 +99,25 @@ apply eqStateRzTrans with (b := b); auto with stalmarck.
 intros a b c S H' H'0 a0 b0.
 apply eqStateRzContr with (a := a); auto with stalmarck.
 Qed.
+
 #[export] Hint Resolve eqStateaddEq1 eqStateaddEq2 : stalmarck.
 
-(* We define the fact of being included *)
-
+(** We define the fact of being included *)
 Definition inclState (S1 S2 : State) : Prop :=
   forall i j : rZ, eqStateRz S1 i j -> eqStateRz S2 i j.
 
 Theorem inclStateRef : forall S : State, inclState S S.
+Proof.
 red in |- *; auto with stalmarck.
 Qed.
-#[export] Hint Resolve inclStateRef : stalmarck.
-(*Simpler version *)
 
+#[export] Hint Resolve inclStateRef : stalmarck.
+
+(** Simpler version *)
 Theorem inclStateIn :
  forall S1 S2 : State,
  (forall a b : rZ, In (a, b) S1 -> eqStateRz S2 a b) -> inclState S1 S2.
+Proof.
 intros S1 S2 H'; red in |- *.
 intros i j H'0; generalize H'; elim H'0; auto with stalmarck.
 intros a b L0 H'1 H'2 H'3; apply eqStateRzSym; auto with stalmarck.
@@ -116,48 +126,57 @@ intros a b c0 L0 H'1 H'2 H'3 H'4 H'5; apply eqStateRzTrans with (b := b);
 intros a b c0 L0 H'1 H'2 H'3; apply eqStateRzContr with (a := a); auto with stalmarck.
 Qed.
 
-(* We define the fact of being equal *)
-
+(** We define the fact of being equal *)
 Definition eqState (S1 S2 : State) : Prop :=
   inclState S1 S2 /\ inclState S2 S1.
 
 Theorem eqStateRef : forall S : State, eqState S S.
+Proof.
 intros; red in |- *; split; auto with stalmarck.
 Qed.
+
 #[export] Hint Resolve eqStateRef : stalmarck.
 
 Theorem eqStateSym : forall S1 S2 : State, eqState S1 S2 -> eqState S2 S1.
+Proof.
 intros S1 S2 H'; elim H'; red in |- *; auto with stalmarck.
 Qed.
+
 #[export] Hint Immediate eqStateSym : stalmarck.
 
 Theorem eqStateInv :
  forall (S1 S2 : State) (a b : rZ),
  eqState S1 S2 -> (eqStateRz S1 a b <-> eqStateRz S2 a b).
+Proof.
 intros S1 S2 a b H'; inversion H'; red in |- *; auto with stalmarck.
 Qed.
 
 Theorem addEqInclState :
  forall (S : State) (a b : rZ), inclState S (addEq (a, b) S).
+Proof.
 intros S a b; red in |- *; auto with stalmarck.
 Qed.
+
 #[export] Hint Resolve addEqInclState : stalmarck.
 
 Theorem inclStateTrans :
  forall S1 S2 S3 : State,
  inclState S1 S2 -> inclState S2 S3 -> inclState S1 S3.
+Proof.
 intros S1 S2 S3 H' H'0; red in |- *; auto with stalmarck.
 Qed.
 
 Theorem eqStateIncl :
  forall (S1 S2 : State) (p q : rZ),
  inclState S1 S2 -> eqStateRz S1 p q -> eqStateRz S2 p q.
+Proof.
 intros S1 S2 p q H' H'0; auto with stalmarck.
 Qed.
 
 Theorem eqStateEq :
  forall (S1 S2 : State) (p q : rZ),
  eqState S1 S2 -> eqStateRz S1 p q -> eqStateRz S2 p q.
+Proof.
 intros S1 S2 p q H' H'0.
 apply eqStateIncl with (S1 := S1); auto with stalmarck.
 inversion H'; auto with stalmarck.
@@ -166,14 +185,17 @@ Qed.
 Theorem addEqInclState2 :
  forall (S : State) (a b c d : rZ),
  inclState S (addEq (a, b) (addEq (c, d) S)).
+Proof.
 intros S a b c d.
 apply inclStateTrans with (S2 := addEq (c, d) S); auto with stalmarck.
 Qed.
+
 #[export] Hint Resolve addEqInclState2 : stalmarck.
 
 Theorem inclStateAddEqInv :
  forall (p q : rZ) (S1 S2 : State),
  inclState S1 S2 -> eqStateRz S2 p q -> inclState (addEq (p, q) S1) S2.
+Proof.
 intros p0 q0 S1 S2 H' H'0; red in |- *; auto with stalmarck.
 intros i j H'1; generalize H'0 H'; auto with stalmarck.
 cut (exists S3 : State, S3 = addEq (p0, q0) S1); auto with stalmarck.
@@ -189,11 +211,13 @@ intros a b c S H'2 H'3 H'4 H'5 H'6.
 apply eqStateRzContr with (a := a); auto with stalmarck.
 exists (addEq (p0, q0) S1); auto with stalmarck.
 Qed.
+
 #[export] Hint Resolve inclStateAddEqInv : stalmarck.
 
 Theorem inclStateAddEq :
  forall (S1 S2 : State) (a b : rZ),
  inclState S1 S2 -> inclState (addEq (a, b) S1) (addEq (a, b) S2).
+Proof.
 intros S1 S2 a b H'.
 apply inclStateAddEqInv; simpl in |- *.
 apply inclStateTrans with (S2 := S2); auto with stalmarck.
@@ -201,18 +225,22 @@ apply eqStateRzIn; auto with stalmarck.
 simpl in |- *.
 auto with stalmarck.
 Qed.
+
 #[export] Hint Resolve inclStateAddEq : stalmarck.
 
 Theorem eqStateAddEq :
  forall (S1 S2 : State) (a b : rZ),
  eqState S1 S2 -> eqState (addEq (a, b) S1) (addEq (a, b) S2).
+Proof.
 intros S1 S2 a b H'; inversion H'; red in |- *; auto with stalmarck.
 Qed.
+
 #[export] Hint Resolve eqStateAddEq : stalmarck.
 
 Theorem inclStateEqStateComp :
  forall S1 S2 S3 S4 : State,
  eqState S1 S2 -> eqState S3 S4 -> inclState S1 S3 -> inclState S2 S4.
+Proof.
 intros S1 S2 S3 S4 H' H'0 H'1; inversion H'; inversion H'0.
 apply inclStateTrans with (S2 := S3); auto with stalmarck.
 apply inclStateTrans with (S2 := S1); auto with stalmarck.
@@ -220,6 +248,7 @@ Qed.
 
 Theorem eqStateTrans :
  forall S1 S2 S3 : State, eqState S1 S2 -> eqState S2 S3 -> eqState S1 S3.
+Proof.
 intros S1 S2 S3 H' H'0; inversion H'; inversion H'0.
 red in |- *; split; apply inclStateTrans with (S2 := S2); auto with stalmarck.
 Qed.
@@ -228,6 +257,7 @@ Theorem addEqComp :
  forall (a b a' b' : rZ) (S : State),
  eqStateRz S a a' ->
  eqStateRz S b b' -> eqState (addEq (a, b) S) (addEq (a', b') S).
+Proof.
 intros a b a' b' S H' H'0.
 red in |- *; split; apply inclStateIn; simpl in |- *;
  (intros a0 b0 H'1; Elimc H'1; intros H'1; [ inversion H'1 | idtac ]); 
@@ -237,30 +267,34 @@ apply eqStateRzTrans with (b := b'); auto with stalmarck.
 apply eqStateRzTrans with (b := a); auto with stalmarck.
 apply eqStateRzTrans with (b := b); auto with stalmarck.
 Qed.
+
 #[export] Hint Resolve addEqComp : stalmarck.
 
-(* A valuation function realizes a state if all its basic equations are true *)
-
+(** A valuation function realizes a state if all its basic equations are true *)
 Definition realizeState (f : rNat -> bool) (S : State) : Prop :=
   forall i j : rZ, In (i, j) S -> rZEval f i = rZEval f j.
 
 Theorem realizeStateNil : forall f : rNat -> bool, realizeState f nil.
+Proof.
 intros f; red in |- *; simpl in |- *.
 intros i j H'; elim H'.
 Qed.
+
 #[export] Hint Resolve realizeStateNil : stalmarck.
 
 Theorem rZEvalCompInv :
  forall (a : rZ) (f : rNat -> bool), rZEval f (rZComp a) = negb (rZEval f a).
+Proof.
 intros a f; case a; simpl in |- *; auto with stalmarck.
 intros r; case (f r); auto with stalmarck.
 Qed.
-(* If a valuation function realizes a state then all its equations are true *)
 
+(** If a valuation function realizes a state then all its equations are true *)
 Theorem realizeStateInv :
  forall (f : rNat -> bool) (S : State),
  realizeState f S ->
  forall i j : rZ, eqStateRz S i j -> rZEval f i = rZEval f j.
+Proof.
 intros f S H' i j H'0; generalize H'; elim H'0; auto with stalmarck.
 intros a b S0 H'1 H'2 H'3.
 rewrite rZEvalCompInv; auto with stalmarck; rewrite rZEvalCompInv; auto with stalmarck.
@@ -279,6 +313,7 @@ Theorem realizeStateInvComp :
  forall (f : rNat -> bool) (S : State),
  realizeState f S ->
  forall i j : rZ, eqStateRz S i (rZComp j) -> rZEval f i = negb (rZEval f j).
+Proof.
 intros f S H' i j H'0.
 rewrite <- rZEvalCompInv.
 apply realizeStateInv with (S := S); auto with stalmarck.
@@ -288,17 +323,20 @@ Theorem realizeStateAddEq :
  forall (f : rNat -> bool) (S : State),
  realizeState f S ->
  forall i j : rZ, rZEval f i = rZEval f j -> realizeState f (addEq (i, j) S).
+Proof.
 intros f S H' i j H'0; red in |- *; simpl in |- *; auto with stalmarck.
 intros i0 j0 H'1; elim H'1; intros H'2; clear H'1; [ inversion H'2 | idtac ];
  auto with stalmarck.
 rewrite <- H1; auto with stalmarck.
 rewrite <- H0; auto with stalmarck.
 Qed.
+
 #[export] Hint Resolve realizeStateAddEq : stalmarck.
 
 Theorem realizeStateIncl :
  forall (f : rNat -> bool) (S1 S2 : State),
  realizeState f S1 -> inclState S2 S1 -> realizeState f S2.
+Proof.
 intros f S1 S2 H' H'0; red in |- *; auto with stalmarck.
 intros i j H'1.
 apply realizeStateInv with (S := S1); auto with stalmarck.
@@ -307,6 +345,7 @@ Qed.
 Theorem realizeStateInvAddEq :
  forall (f : rNat -> bool) (S : State) (i j : rZ),
  realizeState f (addEq (i, j) S) -> rZEval f i = rZEval f j.
+Proof.
 intros f S i j H'.
 apply realizeStateInv with (S := addEq (i, j) S); auto with stalmarck.
 Qed.
@@ -315,33 +354,37 @@ Theorem realizeStateInvAddEq2 :
  forall (f : rNat -> bool) (S : State) (i j k l : rZ),
  realizeState f (addEq (i, j) (addEq (k, l) S)) ->
  rZEval f k = rZEval f l /\ rZEval f i = rZEval f j.
+Proof.
 intros f S i j k l H'; split.
 apply realizeStateInvAddEq with (S := S); auto with stalmarck.
 apply realizeStateIncl with (S1 := addEq (i, j) (addEq (k, l) S)); auto with stalmarck.
 apply realizeStateInvAddEq with (S := addEq (k, l) S); auto with stalmarck.
 Qed.
 
-(* What it means for a state to be contradictory *)
-
+(** What it means for a state to be contradictory *)
 Definition contradictory (S : State) : Prop :=
   exists a : rZ, eqStateRz S a (rZComp a).
-(* Of course if a state is contradictory it can't be realized *)
 
+(** Of course if a state is contradictory it can't be realized *)
 Theorem contradictoryNotRealize :
  forall S : State,
  contradictory S -> forall f : rNat -> bool, ~ realizeState f S.
+Proof.
 intros S H' f; red in |- *; intros H'0; inversion H'.
 absurd (rZEval f x = rZEval f (rZComp x)).
 rewrite rZEvalCompInv; case (rZEval f x); auto with stalmarck; red in |- *; intros;
  discriminate.
 apply realizeStateInv with (S := S); auto with stalmarck.
 Qed.
+
 #[export] Hint Resolve contradictoryNotRealize : stalmarck.
 
 Theorem ContrIncl :
  forall S : State, inclState S ((rZPlus zero, rZMinus zero) :: nil).
+Proof.
 intros S; red in |- *; auto with stalmarck.
 intros i j H'.
 apply eqStateRzContr with (a := rZPlus zero); auto with datatypes stalmarck.
 Qed.
+
 #[export] Hint Resolve ContrIncl : stalmarck.
