theories/unionState.v
@@ -23,8 +23,7 @@ Definition of the union of two states
 From Coq Require Import List.
 From Stalmarck Require Export state.
 
-(* The property of being an union *)
-
+(** The property of being an union *)
 Inductive unionStateP : State -> State -> State -> Prop :=
     unionStatePDef :
       forall S1 S2 S3 : State,
@@ -33,14 +32,17 @@ Inductive unionStateP : State -> State -> State -> Prop :=
       (forall S4 : State,
        inclState S1 S4 -> inclState S2 S4 -> inclState S3 S4) ->
       unionStateP S1 S2 S3.
+
 #[export] Hint Resolve unionStatePDef : stalmarck.
 
 Theorem unionStatePRef : forall S1 : State, unionStateP S1 S1 S1.
+Proof.
 auto with stalmarck.
 Qed.
 
 Theorem unionStatePSym :
  forall S1 S2 S3 : State, unionStateP S1 S2 S3 -> unionStateP S2 S1 S3.
+Proof.
 intros S1 S2 S3 H'; inversion H'; auto with stalmarck.
 Qed.
 
@@ -48,11 +50,13 @@ Theorem unionStatePIncl :
  forall S1 S2 S3 S4 : State,
  unionStateP S1 S2 S3 ->
  inclState S1 S4 -> inclState S2 S4 -> inclState S3 S4.
+Proof.
 intros S1 S2 S3 S4 H' H'0 H'1; inversion H'; auto with stalmarck.
 Qed.
 
 Theorem unionStatePInclSelf :
  forall S1 S2 : State, inclState S2 S1 -> unionStateP S1 S2 S1.
+Proof.
 auto with stalmarck.
 Qed.
 
@@ -61,6 +65,7 @@ Theorem unionStatePEq :
  unionStateP S1 S2 S3 ->
  unionStateP S'1 S'2 S'3 ->
  eqState S1 S'1 -> eqState S2 S'2 -> eqState S3 S'3.
+Proof.
 intros S1 S2 S'1 S'2 S3 S'3 H' H'0; inversion H'; inversion H'0; auto with stalmarck.
 intros H'1 H'2; red in |- *; split; auto with stalmarck.
 apply H1; auto with stalmarck.
@@ -76,6 +81,7 @@ Theorem unionStatePEqComp :
  unionStateP S1 S2 S3 ->
  eqState S1 S'1 ->
  eqState S2 S'2 -> eqState S3 S'3 -> unionStateP S'1 S'2 S'3.
+Proof.
 intros S1 S2 S3 S'1 S'2 S'3 H' H'0 H'1 H'2.
 apply unionStatePDef; auto with stalmarck.
 apply inclStateEqStateComp with (S1 := S1) (S3 := S3); auto with stalmarck.
@@ -94,6 +100,7 @@ Theorem unionStateAssoc1 :
  forall S1 S2 S3 S'1 S'2 S'3 : State,
  unionStateP S1 S2 S'1 ->
  unionStateP S'1 S3 S'2 -> unionStateP S2 S3 S'3 -> unionStateP S1 S'3 S'2.
+Proof.
 intros S1 S2 S3 S'1 S'2 S'3 H' H'0 H'1.
 apply unionStatePDef; auto with stalmarck.
 apply inclStateTrans with (S2 := S'1); auto with stalmarck.
@@ -117,6 +124,7 @@ Theorem unionStatePAssoc2 :
  forall S1 S2 S3 S'1 S'2 S'3 : State,
  unionStateP S2 S3 S'1 ->
  unionStateP S1 S'1 S'2 -> unionStateP S1 S2 S'3 -> unionStateP S'3 S3 S'2.
+Proof.
 intros S1 S2 S3 S'1 S'2 S'3 H' H'0 H'1.
 apply unionStatePDef; auto with stalmarck.
 apply unionStatePIncl with (1 := H'1); auto with stalmarck.
@@ -139,18 +147,19 @@ Qed.
 Theorem addEqUnion :
  forall (S : State) (p q : rZ),
  unionStateP ((p, q) :: nil) S (addEq (p, q) S).
+Proof.
 intros S p q.
 apply unionStatePDef; auto with stalmarck.
 apply inclStateIn; simpl in |- *; auto with stalmarck.
 intros a b H'; elim H'; intros H'0; inversion H'0; auto with stalmarck.
 Qed.
 
-(* To compute of two states, one simply needs to append the two list of equations *)
-
+(** To compute of two states, one simply needs to append the two list of equations *)
 Definition unionState (S1 S2 : State) := S1 ++ S2.
 
 Theorem unionStatePunionState :
  forall S1 S2 : State, unionStateP S1 S2 (unionState S1 S2).
+Proof.
 intros S1; elim S1; simpl in |- *; auto with stalmarck.
 intros S2.
 apply unionStatePSym; auto with stalmarck.
@@ -168,21 +177,26 @@ Qed.
 
 Theorem unionStateInclL :
  forall S1 S2 : State, inclState S1 (unionState S1 S2).
+Proof.
 intros S1 S2.
 destruct (unionStatePunionState S1 S2); auto with stalmarck.
 Qed.
+
 #[export] Hint Resolve unionStateInclL : stalmarck.
 
 Theorem unionStateInclR :
  forall S1 S2 : State, inclState S2 (unionState S1 S2).
+Proof.
 intros S1 S2.
 destruct (unionStatePunionState S1 S2); auto with stalmarck.
 Qed.
+
 #[export] Hint Resolve unionStateInclR : stalmarck.
 
 Theorem unionStateMin :
  forall S1 S2 S3 : State,
  inclState S1 S3 -> inclState S2 S3 -> inclState (unionState S1 S2) S3.
+Proof.
 intros S1 S2 S3 H' H'0.
 destruct (unionStatePunionState S1 S2); auto with stalmarck.
 Qed.
@@ -192,12 +206,14 @@ Theorem unionStateSym :
  forall S1 S2 : State, eqState (unionState S1 S2) (unionState S2 S1).
 intros S1 S2; red in |- *; split; auto with stalmarck.
 Qed.
+
 #[export] Hint Immediate unionStateSym : stalmarck.
 
 Theorem unionStateEq :
  forall S1 S2 S3 S4 : State,
  eqState S1 S3 ->
  eqState S2 S4 -> eqState (unionState S1 S2) (unionState S3 S4).
+Proof.
 intros S1 S2 S3 S4 H' H'0; red in |- *; split; auto with stalmarck.
 apply unionStateMin; auto with stalmarck.
 apply inclStateEqStateComp with (S1 := S3) (S3 := unionState S3 S4); auto with stalmarck.
@@ -206,12 +222,14 @@ apply unionStateMin; auto with stalmarck.
 apply inclStateEqStateComp with (S1 := S1) (S3 := unionState S1 S2); auto with stalmarck.
 apply inclStateEqStateComp with (S1 := S2) (S3 := unionState S1 S2); auto with stalmarck.
 Qed.
+
 #[export] Hint Resolve unionStateEq : stalmarck.
 
 Theorem unionStateAssoc :
  forall S1 S2 S3 : State,
  eqState (unionState S1 (unionState S2 S3))
    (unionState (unionState S1 S2) S3).
+Proof.
 intros S1 S2 S3; red in |- *; split.
 apply unionStateMin; auto with stalmarck.
 apply inclStateTrans with (S2 := unionState S1 S2); auto with stalmarck.
@@ -222,4 +240,5 @@ apply unionStateMin; auto with stalmarck.
 apply inclStateTrans with (S2 := unionState S2 S3); auto with stalmarck.
 apply inclStateTrans with (S2 := unionState S2 S3); auto with stalmarck.
 Qed.
+
 #[export] Hint Resolve unionStateMin : stalmarck.
